adding evaluation

bin/Main.ml
@@ -1,0 +1,33 @@
+open Extracted_code.QuineCode
+
+let rec extract_delayed_val d =
+  match d with
+  | Tick d' ->
+    extract_delayed_val (Lazy.force d')
+  | Boom x -> x
+
+let test tm () =
+  print_endline "The Term:";
+  print_endline "========================";
+  print_endline (print_term 0 tm);
+  print_endline "========================";
+  print_endline "The Evaluated Term:";
+  let t = extract_delayed_val
+    (Lazy.force (normalize 0 tm)) in
+  let eval_str = print_term 0 t in
+  print_endline eval_str;
+  print_endline "========================";
+  print_endline "The Quoted Term:";
+  let q = quote 0 0 tm in
+  let quote_str = print_term 0 q in
+  print_endline quote_str;
+  print_endline "========================";
+  print_endline "Equality Check:";
+  let eq = (eval_str = quote_str) in
+  print_endline (if eq then "TRUE" else "FALSE");
+  ()
+
+let main () =
+  test quine ()
+
+let () = main ()
